오....이렇게 점점 작은 goal 로 쪼개 나가는 거...재밌는데?

src/common/Nemonuri.IndexedStackMap.Invariant.fst
@@ -1,12 +1,31 @@
 module Nemonuri.IndexedStackMap.Invariant
 
-include Nemonuri.IndexedStackMap { t as variant_t }
 module FMap = FStar.FiniteMap.Base
+module FMap = FStar.FiniteMap.Base
+module FSet = FStar.FiniteSet.Base
+open FStar.FiniteSet.Ambient
+open FStar.FiniteMap.Ambient
+
+module I = FStar.IntegerIntervals
+private let rec create_indices_set_agg (n: nat) (idx:I.under (n+1)) :
+  Tot (FSet.set int)
+      (decreases n-idx) =
+  match idx = n with
+  | true -> FSet.emptyset #int
+  | false -> FSet.insert idx (create_indices_set_agg n (idx+1))
+
+type indices_set = FSet.set int
+
+let create_indices_set (n:nat) : Tot indices_set = create_indices_set_agg n 0
+
+type indices_map (data_t:Type) = FMap.map int data_t
 
 noeq
 type t (data_t:Type) = {
   count: nat;
-  v: variant_t count data_t
+  map: indices_map data_t
 }
 
-//let variant_elim 
+let indexed_stack_map_predicate (#data_t:Type) (m:t data_t) =
+  FSet.equal (FMap.domain m.map) (create_indices_set m.count)
+
