src/common/Nemonuri.IndexedStackMap.fst
@@ -3,7 +3,8 @@ module Nemonuri.IndexedStackMap
 module I = FStar.IntegerIntervals
 module FMap = FStar.FiniteMap.Base
 module FSet = FStar.FiniteSet.Base
-
+open FStar.FiniteSet.Ambient
+open FStar.FiniteMap.Ambient
 
 private let rec create_indices_set_agg (n: nat) (idx:I.under (n+1)) :
   Tot (FSet.set (I.under n))
@@ -12,16 +13,83 @@ private let rec create_indices_set_agg (n: nat) (idx:I.under (n+1)) :
   | true -> FSet.emptyset #(I.under n)
   | false -> FSet.insert idx (create_indices_set_agg n (idx+1))
 
-let create_indices_set n = create_indices_set_agg n 0
+type indices_set (n:nat) = FSet.set (I.under n)
 
-let indexed_stack_map_predicate (#n:nat) (#data_t:Type) (m:FMap.map (I.under n) data_t) = FSet.equal (FMap.domain m) (create_indices_set n)
+let create_indices_set (n:nat) : Tot (indices_set n) = create_indices_set_agg n 0
 
-open FStar.FiniteSet.Ambient
-open FStar.FiniteMap.Ambient
-let lemma_create_indices_set_zero () = admit ()
+let lemma_create_indices_set_mem (n: nat) (idx:I.under n)
+  : Lemma (ensures FSet.mem idx (create_indices_set n))
+  =
+  assert (n > 0);
+  assert (FSet.mem idx (create_indices_set_agg n idx));
+  let lemma_create_indices_set_subset (idx2: nat{idx2 <= idx}) : 
+    Lemma (ensures FSet.subset (create_indices_set_agg n idx) (create_indices_set_agg n idx2)) =
+    admit ()
+  in
+  lemma_create_indices_set_subset 0
 
-type t n data_t = x:FMap.map (I.under n) data_t {indexed_stack_map_predicate x}
 
+type indices_map (n:nat) (data_t:Type) = FMap.map (I.under n) data_t
+
+let indexed_stack_map_predicate (#n:nat) (#data_t:Type) (m:indices_map n data_t) = FSet.equal (FMap.domain m) (create_indices_set n)
+
+let lemma_create_indices_set_zero () : Lemma (ensures FSet.equal (FSet.emptyset) (create_indices_set 0)) = ()
+
+type t (n:nat) (data_t:Type) = x:indices_map n data_t {indexed_stack_map_predicate x}
 
 let empty (data_t:Type) : Tot (t 0 data_t) = FMap.emptymap #(I.under 0) #data_t
 
+//--- mem property ---
+let lemma_mem #n #data_t (m:t n data_t) (idx:I.under n)
+  : Lemma (ensures FMap.mem idx m)
+  =
+  //--- Goal: `FSet.mem idx (FMap.domain m)` ---
+  let lemma_mem_domain () : Lemma (FSet.mem idx (FMap.domain m)) =
+    //--- Goal: `FSet.mem idx (create_indices_set n)` ---
+    let lemma_mem_create_indices_set () : Lemma (FSet.mem idx (create_indices_set n)) =
+      admit ()
+    in
+    //---|
+    lemma_mem_create_indices_set ()
+  in
+  //---|
+  lemma_mem_domain ()
+
+
+//---|
+
+//--- invariant ---|
+
+module Iv = Nemonuri.IndexedStackMap.Invariant
+
+private let rec to_invarient_indices_map_agg #n #data_t (m:t n data_t) (idx:I.under (n+1)) :
+  Tot (Iv.indices_map data_t)
+      (decreases n-idx) =
+  match idx = n with
+  | true -> FMap.emptymap #int #data_t
+  | false ->
+  let key = idx <: int in
+  lemma_mem m idx;
+  let value = FMap.lookup idx m in
+  FMap.insert key value (to_invarient_indices_map_agg m (idx+1))
+
+let to_invarient_indices_map #n #data_t (m:t n data_t) 
+  : Tot (Iv.indices_map data_t) =
+  to_invarient_indices_map_agg m 0
+
+let to_invarient #n #data_t (m:t n data_t)
+  : Tot (Iv.t data_t) =
+  {
+    count = n;
+    map = to_invarient_indices_map m
+  }
+
+
+//---|
+
+
+//let grow_map #n #data_t (m:FMap.map (I.under n) data_t) : Tot (FMap.map (I.under (n+1)) data_t) =
+
+
+//let push #n #data_t (m:t n data_t) (d:data_t) : Tot (t (n+1) data_t) =
+//  FMap.insert (n+1) d m
